theories/utp_time_rel.thy
@@ -3,6 +3,7 @@ section {* Timed Relations *}
 theory utp_time_rel
 imports
   utp_rea_designs
+  utp_reactive_hoare
 begin
 
 type_synonym '\<alpha> trel = "('\<alpha>, real pos) rdes"
@@ -19,6 +20,10 @@ definition wait_trel :: "(real pos, '\<alpha>) uexpr \<Rightarrow> '\<alpha> tre
 lemma wait_RR_closed [closure]: "wait\<^sub>r n is RR"
   by (rel_auto, metis add_monoid_diff_cancel_left minus_def trace_class.le_iff_add)
     
+lemma st_subst_rea_wait [usubst]:
+  "\<sigma> \<dagger>\<^sub>S wait\<^sub>r n = wait\<^sub>r (\<sigma> \<dagger> n) ;; \<langle>\<sigma>\<rangle>\<^sub>r"
+  by (rel_auto)
+    
 lemma wait_zero: "wait\<^sub>r(0) = II\<^sub>r"
   by (rel_auto)
 
@@ -29,6 +34,14 @@ lemma wait_cond: "wait\<^sub>r(m) ;; (P \<triangleleft> b \<triangleright>\<^sub
   by (rel_auto)
 
 lemma wait_assign: "x \<sharp> m \<Longrightarrow> wait\<^sub>r(m) ;; x :=\<^sub>r v = x :=\<^sub>r v ;; wait\<^sub>r(m)"
+  by (rel_auto)
+    
+lemma wait_hoare_rp [hoare_safe]:
+  "\<lbrace>p\<rbrace>wait\<^sub>r n\<lbrace>p\<rbrace>\<^sub>r"
+  by (rel_auto)
+   
+lemma hoare_rp_wait_comp [hoare_safe]:
+  "\<lbrace>p\<rbrace> Q \<lbrace>r\<rbrace>\<^sub>r \<Longrightarrow> \<lbrace>p\<rbrace> wait\<^sub>r n ;; Q \<lbrace>r\<rbrace>\<^sub>r"
   by (rel_auto)
     
 end
